Lp2lc/Active/DTLC/Proof.lean
@@ -10,9 +10,9 @@ namespace DTLC
 open AST
 open Lp2lc.Active.Util
 
-theorem AdequacyLemma {I : Index} {ByteCode : Type}
-    [Compiletime.Env I ByteCode] [Runtime.Env I ByteCode]
-    (src : Trm I ByteCode) (fuel : Nat) :
+theorem AdequacyLemma {impl : Impl}
+    [Compiletime.Env impl] [Runtime.Env impl]
+    (src : Trm impl) (fuel : Nat) :
     src.IsAdequate fuel := sorry
 
 
